ground_zero/HITs/join.lean
@@ -1,5 +1,6 @@
-import ground_zero.HITs.pushout
+import ground_zero.HITs.suspension
 open ground_zero.types.product (pr₁ pr₂)
+open ground_zero.types.dep_path (pathover_of_eq)
 
 hott theory
 
@@ -25,6 +26,27 @@ namespace join
     Π (x : join α β), π x :=
   pushout.ind inl₁ inr₁
     (begin intro x, cases x with u v, exact push₁ u v end)
+
+  def rec {π : Type w} (inlπ : α → π) (inrπ : β → π)
+    (pushπ : Π a b, inlπ a = inrπ b) : join α β → π :=
+  ind inlπ inrπ (λ a b, pathover_of_eq (push a b) (pushπ a b))
+
+  def from_susp : ∑α → join bool α :=
+  suspension.rec (inl ff) (inl tt)
+    (λ x, push ff x ⬝ (push tt x)⁻¹)
+
+  def to_susp : join bool α → ∑α :=
+  rec (begin intro x, cases x,
+        exact suspension.north,
+        exact suspension.south
+      end)
+      (λ _, suspension.south)
+      (begin
+        intros x y, cases x,
+        exact suspension.merid y,
+        reflexivity
+      end)
+
 end join
 
 end ground_zero.HITs
